coq_bak/mltt_type.v
@@ -1,0 +1,183 @@
+From mathcomp Require Import ssreflect ssrbool eqtype ssrnat seq.
+From Coq Require Import ssrfun Classical Utf8.
+Require Export AutosubstSsr ARS mltt_ctx mltt_conf.
+
+Set Implicit Arguments.
+Unset Strict Implicit.
+Unset Printing Implicit Defensive.
+
+Inductive mltt0_type : mltt_ctx -> term -> term -> Prop :=
+| mltt0_axiom Γ l :
+  mltt0_wf Γ ->
+  mltt0_type Γ (Ty l) (Ty l.+1)
+| mltt0_var Γ x A :
+  mltt0_wf Γ ->
+  mltt_has Γ x A ->
+  mltt0_type Γ (Var x) A
+| mltt0_pi Γ A B l1 l2 :
+  mltt0_type Γ A (Ty l1) ->
+  mltt0_type (A :: Γ) B (Ty l2) ->
+  mltt0_type Γ (Pi A B) (Ty (maxn l1 l2))
+| mltt0_lam Γ A B m l :
+  mltt0_type Γ A (Ty l) ->
+  mltt0_type (A :: Γ) m B ->
+  mltt0_type Γ (Lam A m) (Pi A B)
+| mltt0_app Γ A B m n :
+  mltt0_type Γ m (Pi A B) ->
+  mltt0_type Γ n A ->
+  mltt0_type Γ (App m n) B.[n/]
+| mltt0_sig Γ A B l1 l2 :
+  mltt0_type Γ A (Ty l1) ->
+  mltt0_type (A :: Γ) B (Ty l2) ->
+  mltt0_type Γ (Sig A B) (Ty (maxn l1 l2))
+| mltt0_dpair Γ A B m n :
+  mltt0_type Γ m A ->
+  mltt0_type Γ n B.[m/] ->
+  mltt0_type Γ (DPair m n) (Sig A B)
+| mltt0_letin Γ A B C m n l :
+  mltt0_type (Sig A B :: Γ) C (Ty l) ->
+  mltt0_type Γ m (Sig A B) ->
+  mltt0_type (B :: A :: Γ) n C.[DPair (Var 1) (Var 0) .: ren (+2)] ->
+  mltt0_type Γ (LetIn C m n) C.[m/]
+| mltt0_tuple Γ A B l1 l2 :
+  mltt0_type Γ A (Ty l1) ->
+  mltt0_type Γ B (Ty l2) ->
+  mltt0_type Γ (Tuple A B) (Ty (maxn l1 l2))
+| mltt0_pair Γ A B m n :
+  mltt0_type Γ m A ->
+  mltt0_type Γ n B ->
+  mltt0_type Γ (Pair m n) (Tuple A B)
+| mltt0_fst Γ A B m :
+  mltt0_type Γ m (Tuple A B) ->
+  mltt0_type Γ (Fst m) A
+| mltt0_snd Γ A B m :
+  mltt0_type Γ m (Tuple A B) ->
+  mltt0_type Γ (Snd m) B
+| mltt0_id Γ A m n l :
+  mltt0_type Γ A (Ty l) ->
+  mltt0_type Γ m A ->
+  mltt0_type Γ n A ->
+  mltt0_type Γ (Id A m n) (Ty l)
+| mltt0_refl Γ A m :
+  mltt0_type Γ m A ->
+  mltt0_type Γ (Refl m) (Id A m m)
+| mltt0_rw Γ A B H P m n l :
+  mltt0_type (Id A.[ren (+1)] m.[ren (+1)] (Var 0) :: A :: Γ) B (Ty l) ->
+  mltt0_type  Γ H B.[Refl m,m/] ->
+  mltt0_type Γ P (Id A m n) ->
+  mltt0_type Γ (Rw B H P) B.[P,n/]
+| mltt0_conv Γ A B m l :
+  A === B ->
+  mltt0_type Γ m A ->
+  mltt0_type Γ B (Ty l) ->
+  mltt0_type Γ m B
+
+with mltt0_wf : mltt_ctx -> Prop :=
+| mltt0_wf_nil : mltt0_wf nil
+| mltt0_wf_cons Γ A l :
+  mltt0_wf Γ ->
+  mltt0_type Γ A (Ty l) ->
+  mltt0_wf (A :: Γ).
+
+Scheme mltt0_type_mut := Induction for mltt0_type Sort Prop
+with mltt0_wf_mut := Induction for mltt0_wf Sort Prop.
+
+Lemma mltt0_type_wf Γ m A : mltt0_type Γ m A -> mltt0_wf Γ.
+Proof with eauto. elim=>{Γ m A}... Qed.
+#[global] Hint Resolve mltt0_type_wf.
+
+Reserved Notation "Γ ⊢ m : A" (at level 50, m, A at next level).
+Inductive mltt_type : mltt_ctx -> term -> term -> Prop :=
+| mltt_axiom Γ l :
+  mltt_wf Γ ->
+  Γ ⊢ Ty l : Ty l.+1
+| mltt_var Γ x A :
+  mltt_wf Γ ->
+  mltt_has Γ x A ->
+  Γ ⊢ Var x : A
+| mltt_pi Γ A B l1 l2 :
+  Γ ⊢ A : Ty l1 ->
+  (A :: Γ) ⊢ B : Ty l2 ->
+  Γ ⊢ Pi A B : Ty (maxn l1 l2)
+| mltt_lam Γ A B m :
+  (A :: Γ) ⊢ m : B ->
+  Γ ⊢ Lam A m : Pi A B
+| mltt_app Γ A B m n :
+  Γ ⊢ m : Pi A B ->
+  Γ ⊢ n : A ->
+  Γ ⊢ App m n : B.[n/]
+| mltt_sig Γ A B l1 l2 :
+  Γ ⊢ A : Ty l1 ->
+  (A :: Γ) ⊢ B : Ty l2  ->
+  Γ ⊢ Sig A B : Ty (maxn l1 l2)
+| mltt_dpair Γ A B m n :
+  Γ ⊢ m : A ->
+  Γ ⊢ n : B.[m/] ->
+  Γ ⊢ DPair m n : Sig A B
+| mltt_letin Γ A B C m n l :
+  (Sig A B :: Γ) ⊢ C : Ty l ->
+  Γ ⊢ m : Sig A B ->
+  (B :: A :: Γ) ⊢ n : C.[DPair (Var 1) (Var 0) .: ren (+2)] ->
+  Γ ⊢ LetIn C m n : C.[m/]
+| mltt_tuple Γ A B l1 l2 :
+  Γ ⊢ A : Ty l1 ->
+  Γ ⊢ B : Ty l2 ->
+  Γ ⊢ Tuple A B : Ty (maxn l1 l2)
+| mltt_pair Γ A B m n :
+  Γ ⊢ m : A ->
+  Γ ⊢ n : B ->
+  Γ ⊢ Pair m n : Tuple A B
+| mltt_fst Γ A B m :
+  Γ ⊢ m : Tuple A B ->
+  Γ ⊢ Fst m : A
+| mltt_snd Γ A B m :
+  Γ ⊢ m : Tuple A B ->
+  Γ ⊢ Snd m : B
+| mltt_id Γ A m n l :
+  Γ ⊢ A : Ty l ->
+  Γ ⊢ m : A ->
+  Γ ⊢ n : A ->
+  Γ ⊢ Id A m n : Ty l
+| mltt_refl Γ A m :
+  Γ ⊢ m : A ->
+  Γ ⊢ Refl m : Id A m m
+| mltt_rw Γ A B H P m n l :
+  (Id A.[ren (+1)] m.[ren (+1)] (Var 0) :: A :: Γ) ⊢ B : Ty l ->
+  Γ ⊢ H : B.[Refl m,m/] ->
+  Γ ⊢ P : Id A m n ->
+  Γ ⊢ Rw B H P : B.[P,n/]
+| mltt_conv Γ A B m l :
+  A === B ->
+  Γ ⊢ m : A ->
+  Γ ⊢ B : Ty l ->
+  Γ ⊢ m : B
+where "Γ ⊢ m : A" := (mltt_type Γ m A)
+
+with mltt_wf : mltt_ctx -> Prop :=
+| mltt_wf_nil : mltt_wf nil
+| mltt_wf_cons Γ A l :
+  mltt_wf Γ ->
+  Γ ⊢ A : Ty l ->
+  mltt_wf (A :: Γ).
+
+Scheme mltt_type_mut := Induction for mltt_type Sort Prop
+with mltt_wf_mut := Induction for mltt_wf Sort Prop.
+
+Axiom mltt_sn : forall Γ m A, Γ ⊢ m : A -> sn mltt_step m.
+
+Lemma mltt_type_wf Γ m A : Γ ⊢ m : A -> mltt_wf Γ.
+Proof with eauto.
+  elim=>{Γ m A}...
+  move=>Γ A B m tym wf. inv wf...
+Qed.
+#[global] Hint Resolve mltt_type_wf.
+
+Lemma mltt_mltt0_type Γ m A : Γ ⊢ m : A -> mltt0_type Γ m A.
+Proof with eauto using mltt0_type, mltt0_wf.
+  move:Γ m A. apply:(@mltt_type_mut _ (fun Γ wf => mltt0_wf Γ))...
+  move=>Γ A B m tym ihm.
+  have wf0:=mltt0_type_wf ihm. inv wf0.
+  apply: mltt0_lam...
+  Unshelve. eauto.
+Qed.
+#[global] Hint Resolve mltt_mltt0_type.
