coq_bak/mltt_weak.v
@@ -1,0 +1,166 @@
+From mathcomp Require Import ssreflect ssrbool eqtype ssrnat seq.
+From Coq Require Import ssrfun Classical Utf8.
+Require Export AutosubstSsr ARS mltt_ctx mltt_type mltt_conf.
+
+Set Implicit Arguments.
+Unset Strict Implicit.
+Unset Printing Implicit Defensive.
+
+Inductive mltt_agree_ren : (var -> var) ->
+  mltt_ctx -> mltt_ctx -> Prop :=
+| mltt_agree_ren_nil ξ :
+  mltt_agree_ren ξ nil nil
+| mltt_agree_ren_cons Γ Γ' ξ m l :
+  Γ ⊢ m : Ty l ->
+  mltt_agree_ren ξ Γ Γ' ->
+  mltt_agree_ren (upren ξ) (m :: Γ) (m.[ren ξ] :: Γ')
+| mltt_agree_ren_wk Γ Γ' ξ m l :
+  Γ' ⊢ m : Ty l ->
+  mltt_agree_ren ξ Γ Γ' ->
+  mltt_agree_ren (ξ >>> (+1)) (Γ) (m :: Γ').
+
+Lemma mltt_agree_ren_refl Γ : mltt_wf Γ -> mltt_agree_ren id Γ Γ.
+Proof with eauto using mltt_agree_ren.
+  move=>wf. elim: wf=>{Γ}...
+  move=>Γ A l wf agr tyA.
+  have:(mltt_agree_ren (upren id) (A :: Γ) (A.[ren id] :: Γ))...
+  by asimpl.
+Qed.
+
+Lemma mltt_agree_ren_has Γ Γ' ξ x A :
+  mltt_agree_ren ξ Γ Γ' -> mltt_has Γ x A -> mltt_has Γ' (ξ x) A.[ren ξ].
+Proof with eauto.
+  move=>agr. elim: agr x A=>{Γ Γ' ξ}.
+  { move=>ξ x A hs. inv hs. }
+  { move=>Γ Γ' ξ m l tym agr ih x A hs. inv hs; asimpl.
+    { replace m.[ren (ξ >>> (+1))] with m.[ren ξ].[ren (+1)] by autosubst.
+      constructor. }
+    { replace A0.[ren (ξ >>> (+1))] with A0.[ren ξ].[ren (+1)] by autosubst.
+      constructor... } }
+  { move=>Γ Γ' ξ m l tym agr ih x B /ih hs. asimpl.
+    replace B.[ren (ξ >>> (+1))] with B.[ren ξ].[ren (+1)] by autosubst.
+    constructor... }
+Qed.
+
+Lemma mltt_agree_weak_wf_nil Γ' ξ : mltt_agree_ren ξ nil Γ' -> mltt_wf Γ'.
+Proof with eauto using mltt_wf.
+  move e:(nil)=>Γ agr. elim: agr e=>//{Γ Γ' ξ}...
+Qed.
+
+Lemma mltt_agree_weak_wf_cons Γ Γ' A ξ :
+  mltt_agree_ren ξ (A :: Γ) Γ' -> mltt_wf Γ ->
+  (∀ Γ' ξ, mltt_agree_ren ξ Γ Γ' → mltt_wf Γ') ->
+  (∀ Γ' ξ, mltt_agree_ren ξ Γ Γ' → exists l, Γ' ⊢ A.[ren ξ] : Ty l) ->
+  mltt_wf Γ'.
+Proof with eauto using mltt_wf.
+  move e:(A :: Γ)=>Γ0 agr. elim: agr Γ A e=>//{Γ0 Γ' ξ}...
+  move=>Γ Γ' ξ m l tym agr _ Γ0 A [e1 e2] wf h1 h2; subst.
+  have[l0 tym']:=h2 _ _ agr.
+  apply: mltt_wf_cons...
+Qed.
+
+Lemma mltt_rename Γ Γ' m A ξ :
+  Γ ⊢ m : A -> mltt_agree_ren ξ Γ Γ' -> Γ' ⊢ m.[ren ξ] : A.[ren ξ].
+Proof with eauto using mltt_type, mltt_wf, mltt_agree_ren.
+  move=>tym. move:Γ m A tym Γ' ξ.
+  apply:(@mltt_type_mut _ (fun Γ wf => forall Γ' ξ, mltt_agree_ren ξ Γ Γ' -> mltt_wf Γ'))...
+  { move=>Γ x A wf h hs Γ' ξ agr. asimpl.
+    apply: mltt_var...
+    apply: mltt_agree_ren_has... }
+  { move=>Γ A B l1 l2 tyA ihA tyB ihB Γ' ξ agr. asimpl.
+    have wf:=mltt_type_wf tyB. inv wf.
+    apply: mltt_pi... }
+  { move=>Γ A B m tym ihm Γ' ξ agr. asimpl.
+    have wf:=mltt_type_wf tym. inv wf.
+    apply: mltt_lam... }
+  { move=>Γ A B m n tym ihm tyn ihn Γ' ξ agr. asimpl.
+    replace B.[n.[ren ξ] .: ren ξ] with B.[ren (upren ξ)].[n.[ren ξ]/]
+      by autosubst.
+    have{}ihm:=ihm _ _ agr.
+    have{}ihn:=ihn _ _ agr.
+    apply: mltt_app...
+    asimpl in ihm... }
+  { move=>Γ A B l1 l2 tyA ihA tyB ihB Γ' ξ agr. asimpl.
+    have{}ihA:=ihA _ _ agr.
+    have{}ihB:=ihB _ _ (mltt_agree_ren_cons tyA agr).
+    apply: mltt_sig... }
+  { move=>Γ A B m n tym ihm tyn ihn Γ' ξ agr. asimpl.
+    have{}ihm:=ihm _ _ agr.
+    have{}ihn:=ihn _ _ agr.
+    asimpl in ihn.
+    apply: mltt_dpair...
+    by autosubst. }
+  { move=>Γ A B C m n l tyC ihC tym ihm tyn ihn Γ' ξ agr. asimpl.
+    have wf:=mltt_type_wf tyC. inv wf.
+    have wf:=mltt_type_wf tyn. inv wf. inv H3.
+    have{}ihC:=ihC _ _ (mltt_agree_ren_cons H2 agr).
+    have{}ihm:=ihm _ _ agr.
+    have/ihn{}ihn:mltt_agree_ren (upren (upren ξ)) (B :: A :: Γ)
+      (B.[ren (upren ξ)] :: A.[ren ξ] :: Γ')...
+    asimpl in ihC.
+    asimpl in ihm.
+    replace C.[DPair (Var 1) (Var 0) .: ren (+2)].[ren (upren (upren ξ))]
+      with C.[ren (upren ξ)].[DPair (Var 1) (Var 0) .: ren (+2)]
+        in ihn by autosubst.
+    have:=mltt_letin ihC ihm ihn.
+    by autosubst. }
+  { move=>Γ A B H P m n l tyB ihB tyH ihH tyP ihP Γ' ξ agr. asimpl.
+    have wf:=mltt_type_wf tyB. inv wf. inv H2.
+    have{}ihP:=ihP _ _ agr.
+    have/ihB{}ihB:
+      mltt_agree_ren (upren (upren ξ))
+        (Id A.[ren (+1)] m.[ren (+1)] (Var 0) :: A :: Γ)
+        ((Id A.[ren (+1)] m.[ren (+1)] (Var 0)).[ren (upren ξ)] :: A.[ren ξ] :: Γ')...
+    have{}ihH:=ihH _ _ agr.
+    asimpl in ihP.
+    asimpl in ihB.
+    asimpl in ihH.
+    replace A.[ren (ξ >>> (+1))] with A.[ren ξ].[ren (+1)] in ihB by autosubst.
+    replace m.[ren (ξ >>> (+1))] with m.[ren ξ].[ren (+1)] in ihB by autosubst.
+    have pf:=mltt_rw ihB. asimpl in pf.
+    have:=pf _ _ _ ihH ihP.
+    by autosubst. }
+  { move=>Γ A B m l eq tym ihm tyB ihB Γ' ξ agr.
+    apply: mltt_conv.
+    apply: mltt_conv_subst.
+    apply: eq.
+    by apply: ihm.
+    have:=ihB _ _ agr.
+    asimpl... }
+  { exact: mltt_agree_weak_wf_nil. }
+  { move=>Γ A l wf ih tyA ihA Γ' ξ agr.
+    apply: mltt_agree_weak_wf_cons... }
+Qed.
+
+Lemma mltt_wf_ok Γ x A :
+  mltt_wf Γ -> mltt_has Γ x A -> exists l, Γ ⊢ A : Ty l.
+Proof with eauto using mltt_agree_ren, mltt_agree_ren_refl.
+  move=>wf. elim: wf x A=>{Γ}.
+  { move=>x A hs. inv hs. }
+  { move=>Γ A l wf ih tyA x B hs. inv hs.
+    { exists l.
+      replace (Ty l) with (Ty l).[ren (+1)] by autosubst.
+      apply: mltt_rename... }
+    { have[l0 tyA0]:=ih _ _ H3.
+      exists l0.
+      replace (Ty l0) with (Ty l0).[ren (+1)] by autosubst.
+      apply: mltt_rename... } }
+Qed.
+
+Lemma mltt_weaken Γ m A B l :
+  Γ ⊢ m : A ->
+  Γ ⊢ B : Ty l ->
+  (B :: Γ) ⊢ m.[ren (+1)] : A.[ren (+1)].
+Proof with eauto using mltt_agree_ren, mltt_agree_ren_refl.
+  move=>tym tyB. apply: mltt_rename...
+Qed.
+
+Lemma mltt_eweaken Γ m m' A A' B l :
+  m' = m.[ren (+1)] ->
+  A' = A.[ren (+1)] ->
+  Γ ⊢ m : A ->
+  Γ ⊢ B : Ty l ->
+  (B :: Γ) ⊢ m' : A'.
+Proof with eauto using mltt_agree_ren, mltt_agree_ren_refl.
+  move=>*; subst. apply: mltt_weaken...
+Qed.
