coq_bak/ptr_heap.v
@@ -1,6 +1,6 @@
 From mathcomp Require Import ssreflect ssrbool eqtype ssrnat seq.
 From Coq Require Import ssrfun Classical Utf8.
-From deriving Require Export deriving.
+From deriving Require Import deriving.
 From extructures Require Export ord fset fmap.
 Require Export AutosubstSsr ARS era_type.
 
@@ -8,9 +8,10 @@ Set Implicit Arguments.
 Unset Strict Implicit.
 Unset Printing Implicit Defensive.
 
-Open Scope fset_scope.
+Section Heap.
+
 Declare Scope heap_scope.
-Local Open Scope heap_scope.
+Open Scope heap_scope.
 
 Definition heap := {fmap nat -> term * sort}.
 
@@ -21,75 +22,17 @@ Definition hkey (H : heap) (s : sort) : Prop :=
        | Some (_, L), L => true
        | None, _ => true
        end.
-Notation "H ▷ s" := (hkey H s) (at level 40) : heap_scope.
+Notation "H ▷ s" := (hkey H s) (at level 40).
 
 Definition hmrg (H1 H2 H3 : heap) : Prop :=
   forall l, match H1 l, H2 l, H3 l with
        | Some (m1, U), Some (m2, U), Some (m3, U) => m1 = m2 /\ m2 = m3
        | Some (m1, L), None, Some (m3, L) => m1 = m3
        | None, Some (m2, L), Some (m3, L) => m2 = m3
-       | None, None, None => true
-       | _, _, _ => false
+       | None, None, None => True
+       | _, _, _ => False
        end.
-
-Ltac rsplit := repeat split.
-Ltac rmatch_case :=
-  repeat match goal with
-    | [ |- context[match ?x with _ => _ end] ] => case_eq x
-    | [ |- context[let (_, _) := ?x in _] ] => destruct x
-    | [ |- forall _, _ ] => intro
-    end;
-  intuition; subst=>//=.
-
-Notation "H1 ∘ H2 => H" := (hmrg H1 H2 H) (at level 40) : heap_scope.
-
-Lemma hdomm_bound (H : heap) : exists x, forall l, x < l -> l \notin domm H.
-Proof.
-  move e:(domm H)=>D {H e}. move: D. apply: fset_ind.
-  exists 0=>l _. by rewrite in_fset0.
-  move=>x D0 h0[x0 ih]. exists (maxn x x0)=> l h1.
-  apply/negP=>h2. rewrite gtn_max in h1. move: h1=>/andP[h3 /ih h4]{ih}.
-  move: h2. rewrite in_fsetU=>/orP[|h5].
-  rewrite in_fset1=>/eqP e. subst. rewrite ltnn in h3. by move: h3=>/negP.
-  rewrite h5 in h4. by move: h4=>/negP. 
-Qed.
-
-Lemma hdomm_exist (H : heap) : exists l, l \notin domm H.
-Proof.
-  have[x h]:=hdomm_bound H.
-  have{}h:=h x.+1 (ltnSn _).
-  by exists x.+1.
-Qed.
-
-Lemma remm_setm (H : heap) l v : l \notin domm H -> remm (setm H l v) l = H.
-Proof.
-  move=>h. apply eq_fmap=>x.
-  rewrite remmE. case_eq (x == l)=>[/eqP e|e]; subst.
-  by move: h=>/dommPn->.
-  by rewrite setmE e.
-Qed.
-
-Lemma hkey_setm H m s l : H ▷ s -> setm H l (m, U) ▷ s.
-Proof.
-  move=>k l0.
-  rewrite setmE. case_eq (l0 == l)=>//.
-Qed.
-
-Lemma hkey_remm H l s : H ▷ s -> remm H l ▷ s.
-Proof.
-  move=>k x.
-  rewrite remmE.
-  case_eq (x == l)=>//.
-Qed.
-
-Lemma hkey_unionm H1 H2 s :
-  domm H1 :#: domm H2 -> H1 ▷ s -> H2 ▷ U -> unionm H1 H2 ▷ s.
-Proof.
-  move=>d k1 k2 l.
-  rewrite unionmE.
-  have:=k1 l. have:=k2 l.
-  rmatch_case.
-Qed.
+Notation "H1 ∘ H2 => H" := (hmrg H1 H2 H) (at level 40).
 
 Lemma hkey_impure H : H ▷ L.
 Proof. move=>l. case (H l)=>//p. case p=>m[|]//. Qed.
@@ -98,77 +41,13 @@ Lemma hkey_merge H1 H2 H s : H1 ∘ H2 => H -> H1 ▷ s -> H2 ▷ s -> H ▷ s.
 Proof.
   move=>mrg k1 k2 l.
   have:=k1 l. have:=k2 l. have:=mrg l.
-  rmatch_case.
-Qed.
-
-Lemma hmrg_none H1 H2 H l :
-  H1 ∘ H2 => H -> l \notin domm H -> l \notin domm H1 /\ l \notin domm H2.
-Proof.
-  move=>mrg/dommPn h1. split; apply/dommPn.
-  move: (mrg l). rewrite h1. by rmatch_case.
-  move: (mrg l). rewrite h1. by rmatch_case.
-Qed.
-
-Lemma hmrg_domm H1 H2 H l :
-  H1 ∘ H2 => H -> l \in domm H1 -> l \in domm H.
-Proof.
-  move=>mrg/dommP[m e].
-  apply/dommP.
-  have:=mrg l. rewrite e.
-  rmatch_case.
-  by exists (t, U).
-  by exists (t, L).
-Qed.
-
-Lemma hmrg_setmU H1 H2 H m l :
-  H1 ∘ H2 => H -> setm H1 l (m, U) ∘ setm H2 l (m, U) => setm H l (m, U).
-Proof.
-  move=>mrg l0. rewrite!setmE. case_eq (l0 == l)=>//e.
-  by have:=mrg l0.
-Qed.
-
-Lemma hmrg_setmL H1 H2 H m l :
-  l \notin domm H -> H1 ∘ H2 => H -> setm H1 l (m, L) ∘ H2 => setm H l (m, L).
-Proof.
-  move=>h0 mrg l0. rewrite!setmE. case_eq (l0 == l)=>[/eqP e|e]; subst.
-  by have[_/dommPn->]:=hmrg_none mrg h0.
-  by have:=mrg l0.
-Qed.
-
-Lemma hmrg_unionm H0 H1 H2 H :
-  H0 ▷ U -> domm H :#: domm H0 -> H1 ∘ H2 => H -> unionm H1 H0 ∘ unionm H2 H0 => unionm H H0.
-Proof.
-  move=>k d mrg l. rewrite!unionmE.
-  case_eq (H1 l); case_eq (H2 l)=>//=.
-  { have:=mrg l. rmatch_case.
-    inv H19. by inv H22.
-    inv H19. by inv H6. }
-  { have:=mrg l. rmatch_case.
-    { move: d=>/fdisjointP h.
-      have h0:H l. by rewrite H12.
-      rewrite-mem_domm in h0.
-      have{h h0}/dommPn e:=h _ h0.
-      rewrite e in H5. by inv H5. }
-    { move: d=>/fdisjointP h.
-      have h0:H l. by rewrite H8.
-      rewrite-mem_domm in h0.
-      have{h h0}/dommPn e:=h _ h0.
-      rewrite e in H5. by inv H5. }
-    { inv H19. by inv H7. } }
-  { have:=mrg l. rmatch_case.
-    { move: d=>/fdisjointP h.
-      have h0:H l. by rewrite H12.
-      rewrite-mem_domm in h0.
-      have{h h0}/dommPn e:=h _ h0.
-      rewrite e in H5. by inv H5. }
-    { move: d=>/fdisjointP h.
-      have h0:H l. by rewrite H8.
-      rewrite-mem_domm in h0.
-      have{h h0}/dommPn e:=h _ h0.
-      rewrite e in H5. by inv H5. }
-    { inv H18. by inv H7. } }
-  { have:=mrg l. rmatch_case.
-    have:=k l. by rewrite H6. }
+  case_eq (H l); case_eq (H2 l); case_eq (H1 l)=>//.
+  { move=>p1 e1 p2 e2 p e.
+    by case: p e; case: p2 e2; case: p1 e1=>m1[|]e1 m2[|]e2 m0[|]e0=>//. }
+  { move=>e1 p2 e2 p e.
+    by case: p e; case: p2 e2=>m2[|]e2 m0[|]e0=>//. }
+  { move=>p1 e1 p2 p e.
+    by case: p e; case: p1 e1=>m1[|]e1 m0[|]e0=>//. }
 Qed.
 
 Lemma hmrg_pure_refl H : H ▷ U -> H ∘ H => H.
@@ -192,7 +71,9 @@ Proof.
   move=>mrg l.
   have:=mrg l.
   case_eq (H l); case_eq (H2 l); case_eq (H1 l)=>//.
-  rmatch_case.
+  { move=>p1 e1 p2 e2 p e.
+    case: p e; case: p2 e2; case: p1 e1=>m1[|]e1 m2[|]e2 m0[|]e0//.
+    by move=>[->->]. }
   { move=>p1 e1 p2 e2 e.
     case: p2 e2; case: p1 e1=>m1[|]e1 m2[|]e2//. }
 Qed.
@@ -206,7 +87,9 @@ Proof.
   move=>l.
   have:=mrg l. have:=k l.
   case_eq (H l); case_eq (H2 l); case_eq (H1 l)=>//.
-  rmatch_case.
+  { move=>p1 e1 p2 e2 p e.
+    case: p e; case: p2 e2; case: p1 e1=>m1[|]e1 m2[|]e2 m0[|]e0//.
+    by move=>_[<-->]. }
   { move=>e1 p2 e2 p e.
     case: p e; case: p2 e2=>m2[|]e2 m0[|]e0=>//.
     by move=>_->. }
@@ -232,7 +115,14 @@ Lemma hmrg_splitL H1 H2 H Ha Hb :
 Proof.
   move=>mrg1 mrg2. exists (unionm Ha H2). split.
   { move=>l.
-    have:=mrg1 l. have:=mrg2 l. rmatch_case.
+    have:=mrg1 l. have:=mrg2 l.
+    (repeat match goal with
+       | [ |- context[match ?x with _ => _ end] ] =>
+           case_eq x
+       | [ |- context[let (_, _) := ?x in _] ] => destruct x
+       | [ |- forall _, _ ] => intro
+       end; subst);
+    intuition; subst=>//.
     all: repeat match goal with
            | [ H1 : context[unionm ?H _], H2 : context[?H] |- _ ] => 
                rewrite unionmE H2 in H1; simpl in H1; inv H1; eauto
@@ -242,7 +132,14 @@ Proof.
                rewrite H1 in H2; inv H2; eauto
            end. }
   { move=>l.
-    have:=mrg1 l. have:=mrg2 l. rmatch_case.
+    have:=mrg1 l. have:=mrg2 l.
+    (repeat match goal with
+       | [ |- context[match ?x with _ => _ end] ] =>
+           case_eq x
+       | [ |- context[let (_, _) := ?x in _] ] => destruct x
+       | [ |- forall _, _ ] => intro
+       end; subst);
+    intuition; subst=>//.
     all: repeat match goal with
            | [ H1 : context[unionm ?H _], H2 : context[?H] |- _ ] => 
                rewrite unionmE H2 in H1; simpl in H1; inv H1; eauto
@@ -298,3 +195,5 @@ Proof.
     case_eq (H l)=>//=p.
     by case: p=>m[|]. }
 Qed.
+  
+End Heap.
