coq_bak/ptr_sr.v
@@ -1,6 +1,6 @@
 From mathcomp Require Import ssreflect ssrbool eqtype ssrnat seq.
 From Coq Require Import ssrfun Classical Utf8.
-Require Export AutosubstSsr ARS era_sr ptr_step ptr_subst.
+Require Export AutosubstSsr ARS ptr_step ptr_subst era_sr.
 
 Set Implicit Arguments.
 Unset Strict Implicit.
@@ -12,87 +12,65 @@ Lemma ptr_srX H1 H2 H H' x y z z' A :
   exists H1' H2' x' y',
     H1' ; x' ~ y' ~ z' : A /\ wr_heap H' /\
     pad H2 H2' /\ H1' ∘ H2' => H' /\ x ~>>* x' /\ y ~>>* y'.
-Proof with eauto 7 using era_type, resolve, dyn_step, key, merge, hmrg_setmU, hmrg_setmL, pad_refl.
+Proof with eauto 7 using pad, era_type, resolve, merge, free, key, dyn_step.
   move=>{H1 x y z A}[H1 x y z A].
   move e1:(nil)=>Γ. move e2:(nil)=>Δ er.
   elim: er H1 H2 H H' z z' e1 e2=>{Γ Δ x y A}.
   { move=>Γ Δ x s A wf shs dhs H1 H2 H H' z z' e1 e2 rs wr mrg st; subst. inv shs. }
   { move=>Γ Δ A B m m' s k erm _ H1 H2 H H' z z' e1 e2 rs wr mrg st; subst.
     inv rs; inv st.
+    have[<-_]:=merge_size mrg.
     have[wr1 wr2]:=wr_merge_inv mrg wr.
     destruct s.
-    { exists (setm H1 l (Lam0 Box m0 U, U)).
-      exists (setm H2 l (Lam0 Box m0 U, U)).
+    { exists (Lam0 Box m0 U :U H1).
+      exists (Lam0 Box m0 U :U H2).
       exists (Lam0 A m U).
       exists (Lam0 Box m' U).
-      rsplit...
-      { econstructor.
-        rewrite/free setmE eq_refl. rsplit.
-        apply: resolve_wkU.
+      repeat split...
+      { econstructor...
         constructor...
-        by have[]:=hmrg_none mrg H10. }
-      { have//=nfm':=nf_typing erm.
-        have//=nfm0:=resolve_wr_nfi H8 wr1 nfm'.
-        apply: wr_merge.
-        apply: hmrg_setmU...
-        move=>x. have:=wr1 x. rewrite setmE. by case: eqP.
-        move=>x. have:=wr2 x. rewrite setmE. by case: eqP. }
-      { apply: pad_setm.
-        by have[]:=hmrg_none mrg H10. } }
-    { exists (setm H1 l (Lam0 Box m0 L, L)).
-      exists (H2).
+        apply: resolve_wkU... }
+      { constructor...
+        have//=nfm':=nf_typing erm.
+        have//:=resolve_wr_nfi H8 wr1 nfm'. } }
+    { exists (Lam0 Box m0 L :L H1).
+      exists (_: H2).
       exists (Lam0 A m L).
       exists (Lam0 Box m' L).
-      rsplit...
-      { econstructor.
-        rewrite/free setmE eq_refl. rsplit.
-        rewrite remm_setm.
+      repeat split...
+      { econstructor...
         constructor...
-        by have[]:=hmrg_none mrg H10. }
-      { have//=nfm':=nf_typing erm.
-        have//=nfm0:=resolve_wr_nfi H8 wr1 nfm'.
-        apply: wr_merge.
-        apply: hmrg_setmL...
-        move=>x. have:=wr1 x. rewrite setmE. by case: eqP.
-        exact: wr2. } } }
+        apply: resolve_wkN... }
+      { constructor...
+        have//=nfm':=nf_typing erm.
+        have//:=resolve_wr_nfi H8 wr1 nfm'. } } }
   { move=>Γ Δ A B m m' s t k erm _ H1 H2 H H' z z' e1 e2 rs wr mrg st; subst.
     inv rs; inv st.
+    have[<-_]:=merge_size mrg.
     have[wr1 wr2]:=wr_merge_inv mrg wr.
     destruct s.
-    { exists (setm H1 l (Lam1 Box m0 U, U)).
-      exists (setm H2 l (Lam1 Box m0 U, U)).
+    { exists (Lam1 Box m0 U :U H1).
+      exists (Lam1 Box m0 U :U H2).
       exists (Lam1 A m U).
       exists (Lam1 Box m' U).
-      rsplit...
-      { econstructor.
-        rewrite/free setmE eq_refl. rsplit.
-        apply: resolve_wkU.
+      repeat split...
+      { econstructor...
         constructor...
-        by have[]:=hmrg_none mrg H10. }
-      { have//=nfm':=nf_typing erm.
-        have//=nfm0:=resolve_wr_nfi H8 wr1 nfm'.
-        apply: wr_merge.
-        apply: hmrg_setmU...
-        move=>x. have:=wr1 x. rewrite setmE. by case: eqP.
-        move=>x. have:=wr2 x. rewrite setmE. by case: eqP. }
-      { apply: pad_setm.
-        by have[]:=hmrg_none mrg H10. } }
-    { exists (setm H1 l (Lam1 Box m0 L, L)).
-      exists (H2).
+        apply: resolve_wkU... }
+      { constructor...
+        have//=nfm':=nf_typing erm.
+        have//:=resolve_wr_nfi H8 wr1 nfm'. } }
+    { exists (Lam1 Box m0 L :L H1).
+      exists (_: H2).
       exists (Lam1 A m L).
       exists (Lam1 Box m' L).
-      rsplit...
-      { econstructor.
-        rewrite/free setmE eq_refl. rsplit.
-        rewrite remm_setm.
+      repeat split...
+      { econstructor...
         constructor...
-        by have[]:=hmrg_none mrg H10. }
-      { have//=nfm':=nf_typing erm.
-        have//=nfm0:=resolve_wr_nfi H8 wr1 nfm'.
-        apply: wr_merge.
-        apply: hmrg_setmL...
-        move=>x. have:=wr1 x. rewrite setmE. by case: eqP.
-        exact: wr2. } } }
+        apply: resolve_wkN... }
+      { constructor...
+        have//=nfm':=nf_typing erm.
+        have//:=resolve_wr_nfi H8 wr1 nfm'. } } }
   { move=>Γ Δ A B m m' n s erm ihm tyn H1 H2 H H' z z' e1 e2 rs wr mrg st; subst.
     inv rs; inv st.
     { have[H1'[H2'[x'[y'[wrx[wr'[pd[mrg'[rd1 rd2]]]]]]]]]:=ihm _ _ _ _ _ _ erefl erefl H6 wr mrg H9.
@@ -113,7 +91,7 @@ Proof with eauto 7 using era_type, resolve, dyn_step, key, merge, hmrg_setmU, hm
       { have[ern _]:=era_lam0_inv erm.
         have wr':=free_wr H9 wr.
         have[wr1 wr2]:=wr_merge_inv mrg' wr'.
-        have[Hx[k mrgx]]:=hsplit_self H1'.
+        have[Hx[k mrgx]]:=split_self H1'.
         have[_ wrx]:=wr_merge_inv mrgx wr1.
         apply: resolve_subst...
         constructor.
@@ -139,27 +117,27 @@ Proof with eauto 7 using era_type, resolve, dyn_step, key, merge, hmrg_setmU, hm
     { have//:=era_box_form ern. }
     { have//:=era_box_form ern. }
     { have[wr1 wr2]:=wr_merge_inv mrg2 wr.
-      have[H4[mrg3 mrg4]]:=hmrg_splitR mrg2 H7.
+      have[H4[mrg3 mrg4]]:=merge_splitR mrg2 H7.
       have[H1'[H2'[x'[y'[wrx[wr'[pd[mrg5[rd1 rd2]]]]]]]]]:=
-        ihm _ _ _ _ _ _ erefl erefl H10 wr (hmrg_sym mrg4) H13.
+        ihm _ _ _ _ _ _ erefl erefl H10 wr (merge_sym mrg4) H13.
       have[H1p[H2p[pd1[pd2 mrp]]]]:=pad_merge pd mrg3.
-      have[Hx[mrp1 mrp2]]:=hmrg_splitL (hmrg_sym mrg5) mrp.
+      have[Hx[mrp1 mrp2]]:=merge_splitL (merge_sym mrg5) mrp.
       inv wrx.
       exists Hx. exists H2p. exists (App x' n). exists (App y' n').
       repeat split...
       { econstructor.
-        apply: hmrg_sym...
+        apply: merge_sym...
         apply: H8.
         apply: resolve_pad... }
       { apply: (star_hom (App^~ n)) rd1=>x y.
         apply: dyn_step_appL. }
       { apply: (star_hom (App^~ n')) rd2=>x y.
         apply: dyn_step_appL. } }
-    { have[H4[mrg3 mrg4]]:=hmrg_splitL mrg2 H7.
+    { have[H4[mrg3 mrg4]]:=merge_splitL mrg2 H7.
       have[H1'[H2'[x'[y'[wrx[wr'[pd[mrg5[rd1 rd2]]]]]]]]]:=
-        ihn _ _ _ _ _ _ erefl erefl H11 wr (hmrg_sym mrg4) H13.
+        ihn _ _ _ _ _ _ erefl erefl H11 wr (merge_sym mrg4) H13.
       have[H1p[H2p[pd1[pd2 mrp]]]]:=pad_merge pd mrg3.
-      have[Hx[mrp1 mrp2]]:=hmrg_splitL (hmrg_sym mrg5) mrp.
+      have[Hx[mrp1 mrp2]]:=merge_splitL (merge_sym mrg5) mrp.
       inv wrx.
       exists Hx. exists H2p. exists (App m x'). exists (App m' y').
       repeat split...
@@ -180,19 +158,19 @@ Proof with eauto 7 using era_type, resolve, dyn_step, key, merge, hmrg_setmU, hm
         apply: dyn_step_appR. }
       { apply: (star_hom (App m')) rd2=>x y.
         apply: dyn_step_appR. } }
-    { have[Hx[mrg3 mrg4]]:=hmrg_splitR mrg2 H7.
-      have[Hy[mrg5 rs]]:=resolve_free H13 H10 (hmrg_sym mrg4). inv rs.
+    { have[Hx[mrg3 mrg4]]:=merge_splitR mrg2 H7.
+      have[Hy[mrg5 rs]]:=resolve_free H13 H10 (merge_sym mrg4). inv rs.
       have[A0[n1 e]]:=era_lam0_form erm. subst.
       exfalso. apply: sta_lam0_pi1_false... }
-    { have[H4[mrg3 mrg4]]:=hmrg_splitR mrg2 H7.
-      have[H5[mrg rs]]:=resolve_free H13 H10 (hmrg_sym mrg4). inv rs.
-      have[Hx[mrg5 mrg6]]:=hmrg_splitL (hmrg_sym mrg) mrg3.
+    { have[H4[mrg3 mrg4]]:=merge_splitR mrg2 H7.
+      have[H5[mrg rs]]:=resolve_free H13 H10 (merge_sym mrg4). inv rs.
+      have[Hx[mrg5 mrg6]]:=merge_splitL (merge_sym mrg) mrg3.
       have[A0[n0 e]]:=era_lam1_form erm. subst.
       have[r[ern0 _]]:=era_lam1_inv erm.
       have wr':=free_wr H13 wr.
       have[wr1 wr2]:=wr_merge_inv mrg wr'.
       have[wr3 wr4]:=wr_merge_inv mrg3 wr2.
-      have[H3'[k mrg']]:=hsplit_self H3.
+      have[H3'[k mrg']]:=split_self H3.
       have[_ wr3']:=wr_merge_inv mrg' wr3.
       have vl':=wr_resolve_ptr wr3 H11.
       have vl:=era_dyn_val ern vl'.
@@ -208,30 +186,29 @@ Proof with eauto 7 using era_type, resolve, dyn_step, key, merge, hmrg_setmU, hm
         destruct r.
         { apply: resolve_subst.
           apply: ern0.
-          apply: hmrg_sym...
+          apply: merge_sym...
           apply: H16.
           apply: wr1.
           apply: agree_resolve_wkU.
-          apply: hmrg_sym...
+          apply: merge_sym...
           all: eauto.
           constructor... }
         { apply: resolve_subst.
           apply: ern0.
-          apply: hmrg_sym...
+          apply: merge_sym...
           all: eauto.
           apply: agree_resolve_wkL.
-          apply: hmrg_sym...
+          apply: merge_sym...
           all: eauto.
           constructor... } }
       { apply: star1. apply: dyn_step_beta1... }
       { apply: star1. apply: dyn_step_beta1... } } }
   { move=>Γ Δ A B m m' n t l tyS erm ihm tyn H1 H2 H H' z z' e1 e2 rs wr mrg st; subst.
-    have[wr1 wr2]:=wr_merge_inv mrg wr.
     inv rs; inv st.
     { have[H1'[H2'[x'[y'[wrx[wr'[pd[mrg'[rd1 rd2]]]]]]]]]:=ihm _ _ _ _ _ _ erefl erefl H6 wr mrg H9.
       inv wrx.
       exists H1'. exists H2'. exists (Pair0 x' n t). exists (Pair0 y' Box t).
-      rsplit...
+      repeat split...
       { have[s[r[l1[l2[ord[tyA[tyB _]]]]]]]:=sta_sig0_inv tyS.
         have tyx:=dyn_sta_type (dyn_rd (era_dyn_type erm) rd1).
         have//=tyBx:=sta_subst tyB tyx.
@@ -246,46 +223,34 @@ Proof with eauto 7 using era_type, resolve, dyn_step, key, merge, hmrg_setmU, hm
         apply: dyn_step_pair0L. }
       { apply: (star_hom ((Pair0^~ Box)^~ t)) rd2=>x y.
         apply: dyn_step_pair0L. } }
-    { destruct t.
-      { exists (setm H1 l0 (Pair0 (Ptr lm) Box U, U)).
-        exists (setm H2 l0 (Pair0 (Ptr lm) Box U, U)).
+    { have[e1 e2]:=merge_size mrg. destruct t.
+      { exists (Pair0 (Ptr lm) Box U :U H1).
+        exists (Pair0 (Ptr lm) Box U :U H2).
         exists (Pair0 m n U).
         exists (Pair0 m' Box U).
-        rsplit...
+        repeat split...
         { econstructor.
-          rewrite/free setmE eq_refl. rsplit.
-          apply: resolve_wkU.
           constructor...
-          by have[]:=hmrg_none mrg H9. }
-        { apply: wr_merge.
-          apply: hmrg_setmU...
-          move=>x. have:=wr1 x. rewrite setmE. by case: eqP.
-          move=>x. have:=wr2 x. rewrite setmE. by case: eqP. }
-        { apply: pad_setm.
-          by have[]:=hmrg_none mrg H9. } }
-      { exists (setm H1 l0 (Pair0 (Ptr lm) Box L, L)).
-        exists (H2).
+          constructor.
+          apply: resolve_wkU... }
+        { constructor... } }
+      { exists (Pair0 (Ptr lm) Box L :L H1).
+        exists (_: H2).
         exists (Pair0 m n L).
         exists (Pair0 m' Box L).
-        rsplit...
+        repeat split...
         { econstructor.
-          rewrite/free setmE eq_refl. rsplit.
-          rewrite remm_setm.
           constructor...
-          by have[]:=hmrg_none mrg H9. }
-        { apply: wr_merge.
-          apply: hmrg_setmL...
-          move=>x. have:=wr1 x. rewrite setmE. by case: eqP.
-          exact: wr2. } } } }
+          constructor.
+          apply: resolve_wkN... }
+        { constructor... } } } }
   { move=>Γ Δ1 Δ2 Δ A B m m' n n' t l mrg1 tyS erm ihm ern ihn H1 H2 H H' z z' e1 e2 rs wr mrg2 st; subst.
-    have[s[r[l1[l2[ord1[ord2[tyA[tyB _]]]]]]]]:=sta_sig1_inv tyS. inv mrg1.
-    have[wr1 wr2]:=wr_merge_inv mrg2 wr.
-    inv rs; inv st.
-    { have[H4[mrg3 mrg4]]:=hmrg_splitR mrg2 H10.
+    have[s[r[l1[l2[ord1[ord2[tyA[tyB _]]]]]]]]:=sta_sig1_inv tyS. inv mrg1. inv rs; inv st.
+    { have[H4[mrg3 mrg4]]:=merge_splitR mrg2 H10.
       have[H1'[H2'[x'[y'[wrx[wr'[pd[mrg'[rd1 rd2]]]]]]]]]:=
-        ihm _ _ _ _ _ _ erefl erefl H11 wr (hmrg_sym mrg4) H14. inv wrx.
+        ihm _ _ _ _ _ _ erefl erefl H11 wr (merge_sym mrg4) H14. inv wrx.
       have[H1p[H2p[pd1[pd2 mrp]]]]:=pad_merge pd mrg3.
-      have[Hx[mrp1 mrp2]]:=hmrg_splitL (hmrg_sym mrg') mrp.
+      have[Hx[mrp1 mrp2]]:=merge_splitL (merge_sym mrg') mrp.
       exists Hx. exists H2p. exists (Pair1 x' n t). exists (Pair1 y' n' t).
       repeat split...
       { have tyx:=dyn_sta_type (dyn_rd (era_dyn_type erm) rd1).
@@ -298,18 +263,18 @@ Proof with eauto 7 using era_type, resolve, dyn_step, key, merge, hmrg_setmU, hm
         apply: ern.
         apply: tyBx. }
       { econstructor.
-        apply: hmrg_sym...
+        apply: merge_sym...
         apply: H7.
         apply: resolve_pad... }
       { apply: (star_hom ((Pair1^~ n)^~ t)) rd1=>x y.
         apply: dyn_step_pair1L. }
       { apply: (star_hom ((Pair1^~ n')^~ t)) rd2=>x y.
         apply: dyn_step_pair1L. } }
-    { have[H4[mrg3 mrg4]]:=hmrg_splitL mrg2 H10.
+    { have[H4[mrg3 mrg4]]:=merge_splitL mrg2 H10.
       have[H1'[H2'[x'[y'[wrx[wr'[pd[mrg'[rd1 rd2]]]]]]]]]:=
-        ihn _ _ _ _ _ _ erefl erefl H12 wr (hmrg_sym mrg4) H14. inv wrx.
+        ihn _ _ _ _ _ _ erefl erefl H12 wr (merge_sym mrg4) H14. inv wrx.
       have[H1p[H2p[pd1[pd2 mrp]]]]:=pad_merge pd mrg3.
-      have[Hx[mrp1 mrp2]]:=hmrg_splitL (hmrg_sym mrg') mrp.
+      have[Hx[mrp1 mrp2]]:=merge_splitL (merge_sym mrg') mrp.
       exists Hx. exists H2p. exists (Pair1 m x' t). exists (Pair1 m' y' t).
       repeat split...
       { econstructor...
@@ -318,45 +283,37 @@ Proof with eauto 7 using era_type, resolve, dyn_step, key, merge, hmrg_setmU, hm
         apply: dyn_step_pair1R. }
       { apply: (star_hom (Pair1 m'^~ t)) rd2=>x y.
         apply: dyn_step_pair1R. } }
-    { destruct t.
-      { exists (setm H1 l0 (Pair1 (Ptr lm) (Ptr ln) U, U)).
-        exists (setm H2 l0 (Pair1 (Ptr lm) (Ptr ln) U, U)).
+    { have[e1 e2]:=merge_size mrg2. destruct t.
+      { exists (Pair1 (Ptr lm) (Ptr ln) U :U H1).
+        exists (Pair1 (Ptr lm) (Ptr ln) U :U H2).
         exists (Pair1 m n U).
         exists (Pair1 m' n' U).
-        rsplit...
+        repeat split...
         { econstructor.
-          rewrite/free setmE eq_refl. rsplit.
-          apply: resolve_wkU.
+          constructor...
           econstructor...
-          by have[]:=hmrg_none mrg2 H14. }
-        { apply: wr_merge.
-          apply: hmrg_setmU...
-          move=>x. have:=wr1 x. rewrite setmE. by case: eqP.
-          move=>x. have:=wr2 x. rewrite setmE. by case: eqP. }
-        { apply: pad_setm.
-          by have[]:=hmrg_none mrg2 H14. } }
-      { exists (setm H1 l0 (Pair1 (Ptr lm) (Ptr ln) L, L)).
-        exists (H2).
+          apply: resolve_wkU...
+          apply: resolve_wkU... }
+        { constructor... } }
+      { exists (Pair1 (Ptr lm) (Ptr ln) L :L H1).
+        exists (_: H2).
         exists (Pair1 m n L).
         exists (Pair1 m' n' L).
-        rsplit...
+        repeat split...
         { econstructor.
-          rewrite/free setmE eq_refl. rsplit.
-          rewrite remm_setm.
+          constructor...
           econstructor...
-          by have[]:=hmrg_none mrg2 H14. }
-        { apply: wr_merge.
-          apply: hmrg_setmL...
-          move=>x. have:=wr1 x. rewrite setmE. by case: eqP.
-          exact: wr2. } } } }
+          apply: resolve_wkN...
+          apply: resolve_wkN... }
+        { constructor... } } } }
   { move=>Γ Δ1 Δ2 Δ A B C m m' n n' s r t l mrg1 tyC
       erm ihm ern _ H1 H2 H H' z z' e1 e2 rs wr mrg2 st; subst.
     inv mrg1. inv rs; inv st.
-    { have[H4[mrg3 mrg4]]:=hmrg_splitR mrg2 H7.
+    { have[H4[mrg3 mrg4]]:=merge_splitR mrg2 H7.
       have[H1'[H2'[x'[y'[wrx[wr'[pd[mrg'[rd1 rd2]]]]]]]]]:=
-        ihm _ _ _ _ _ _ erefl erefl H10 wr (hmrg_sym mrg4) H13. inv wrx.
+        ihm _ _ _ _ _ _ erefl erefl H10 wr (merge_sym mrg4) H13. inv wrx.
       have[H1p[H2p[pd1[pd2 mrp]]]]:=pad_merge pd mrg3.
-      have[Hx[mrp1 mrp2]]:=hmrg_splitL (hmrg_sym mrg') mrp.
+      have[Hx[mrp1 mrp2]]:=merge_splitL (merge_sym mrg') mrp.
       exists Hx. exists H2p. exists (LetIn C x' n). exists (LetIn Box y' n').
       repeat split...
       { apply: era_conv.
@@ -368,16 +325,16 @@ Proof with eauto 7 using era_type, resolve, dyn_step, key, merge, hmrg_setmU, hm
         apply: sta_esubst...
         autosubst. }
       { econstructor.
-        apply: hmrg_sym...
+        apply: merge_sym...
         apply: H8.
         apply: resolve_pad... }
       { apply: (star_hom (LetIn C^~ n)) rd1=>x y.
         apply: dyn_step_letinL. }
       { apply: (star_hom (LetIn Box^~ n')) rd2=>x y.
         apply: dyn_step_letinL. } }
-    { have[H4[mrg3 mrg4]]:=hmrg_splitR mrg2 H7.
-      have[H1'[mrg' rs]]:=resolve_free H13 H10 (hmrg_sym mrg4). inv rs.
-      have[Hx[mrg5 mrg6]]:=hmrg_splitL (hmrg_sym mrg') mrg3.
+    { have[H4[mrg3 mrg4]]:=merge_splitR mrg2 H7.
+      have[H1'[mrg' rs]]:=resolve_free H13 H10 (merge_sym mrg4). inv rs.
+      have[Hx[mrg5 mrg6]]:=merge_splitL (merge_sym mrg') mrg3.
       have[m1[m2 e]]:=era_pair0_form erm. subst.
       have[e[_[erm1 tym2]]]:=era_pair0_inv erm. subst.
       have wr':=free_wr H13 wr.
@@ -387,7 +344,7 @@ Proof with eauto 7 using era_type, resolve, dyn_step, key, merge, hmrg_setmU, hm
       have vl:=wr_resolve_ptr wr5 H15.
       have wf:=dyn_type_wf (era_dyn_type ern). inv wf.  inv H9.
       have k1:=resolution (Ptr_well_resolved erm1 H15) H17 vl wr5.
-      have[H2'[k mrg2']]:=hsplit_self H1'.
+      have[H2'[k mrg2']]:=split_self H1'.
       have[_ wr7]:=wr_merge_inv mrg2' wr5.
       exists Hx. exists H2. exists n.[m2,m1/]. exists (n'.[Box,m'0/]).
       repeat split...
@@ -404,13 +361,13 @@ Proof with eauto 7 using era_type, resolve, dyn_step, key, merge, hmrg_setmU, hm
         { apply: resolve_subst...
           constructor.
           econstructor.
-          apply: hmrg_sym mrg2'.
+          apply: merge_sym mrg2'.
           all: eauto.
           constructor... }
         { apply: resolve_subst...
           constructor.
           econstructor.
-          apply: hmrg_sym mrg2'.
+          apply: merge_sym mrg2'.
           all: eauto.
           constructor... } }
       { apply: star1.
@@ -420,18 +377,18 @@ Proof with eauto 7 using era_type, resolve, dyn_step, key, merge, hmrg_setmU, hm
       { apply: star1.
         constructor.
         constructor... } }
-    { have[H4[mrg3 mrg4]]:=hmrg_splitR mrg2 H7.
-      have[H1'[mrg' rs]]:=resolve_free H13 H10 (hmrg_sym mrg4). inv rs.
+    { have[H4[mrg3 mrg4]]:=merge_splitR mrg2 H7.
+      have[H1'[mrg' rs]]:=resolve_free H13 H10 (merge_sym mrg4). inv rs.
       have[m1[m2 e]]:=era_pair1_form erm. subst.
       exfalso. apply: sta_pair1_sig0_false... } }
   { move=>Γ Δ1 Δ2 Δ A B C m m' n n' s r1 r2 t l mrg1 tyC
       erm ihm ern _ H1 H2 H H' z z' e1 e2 rs wr mrg2 st; subst.
     inv mrg1. inv rs; inv st.
-    { have[H4[mrg3 mrg4]]:=hmrg_splitR mrg2 H7.
+    { have[H4[mrg3 mrg4]]:=merge_splitR mrg2 H7.
       have[H1'[H2'[x'[y'[wrx[wr'[pd[mrg'[rd1 rd2]]]]]]]]]:=
-        ihm _ _ _ _ _ _ erefl erefl H10 wr (hmrg_sym mrg4) H13. inv wrx.
+        ihm _ _ _ _ _ _ erefl erefl H10 wr (merge_sym mrg4) H13. inv wrx.
       have[H1p[H2p[pd1[pd2 mrp]]]]:=pad_merge pd mrg3.
-      have[Hx[mrp1 mrp2]]:=hmrg_splitL (hmrg_sym mrg') mrp.
+      have[Hx[mrp1 mrp2]]:=merge_splitL (merge_sym mrg') mrp.
       exists Hx. exists H2p. exists (LetIn C x' n). exists (LetIn Box y' n').
       repeat split...
       { apply: era_conv.
@@ -443,20 +400,20 @@ Proof with eauto 7 using era_type, resolve, dyn_step, key, merge, hmrg_setmU, hm
         apply: sta_esubst...
         autosubst. }
       { econstructor.
-        apply: hmrg_sym...
+        apply: merge_sym...
         apply: H8.
         apply: resolve_pad... }
       { apply: (star_hom (LetIn C^~ n)) rd1=>x y.
         apply: dyn_step_letinL. }
       { apply: (star_hom (LetIn Box^~ n')) rd2=>x y.
         apply: dyn_step_letinL. } }
-    { have[H4[mrg3 mrg4]]:=hmrg_splitR mrg2 H7.
-      have[H1'[mrg' rs]]:=resolve_free H13 H10 (hmrg_sym mrg4). inv rs.
+    { have[H4[mrg3 mrg4]]:=merge_splitR mrg2 H7.
+      have[H1'[mrg' rs]]:=resolve_free H13 H10 (merge_sym mrg4). inv rs.
       have[m1[m2 e]]:=era_pair0_form erm. subst.
       exfalso. apply: sta_pair0_sig1_false... }
-    { have[H4[mrg3 mrg4]]:=hmrg_splitR mrg2 H7.
-      have[H1'[mrg' rs]]:=resolve_free H13 H10 (hmrg_sym mrg4). inv rs.
-      have[Hx[mrg5 mrg6]]:=hmrg_splitL (hmrg_sym mrg') mrg3.
+    { have[H4[mrg3 mrg4]]:=merge_splitR mrg2 H7.
+      have[H1'[mrg' rs]]:=resolve_free H13 H10 (merge_sym mrg4). inv rs.
+      have[Hx[mrg5 mrg6]]:=merge_splitL (merge_sym mrg') mrg3.
       have[m1[m2 e]]:=era_pair1_form erm. subst.
       have[Δ1[Δ2[mrg[e[erm1 erm2]]]]]:=era_pair1_inv erm. inv mrg; subst.
       have wr':=free_wr H13 wr.
@@ -470,8 +427,8 @@ Proof with eauto 7 using era_type, resolve, dyn_step, key, merge, hmrg_setmU, hm
       have k1:=resolution (Ptr_well_resolved erm1 H18) H21 vm wr7.
       have//=tyBm1:=sta_subst H17 (dyn_sta_type (era_dyn_type erm1)).
       have k2:=resolution (Ptr_well_resolved erm2 H19) tyBm1 vn wr8.
-      have[H5'[k5 mrg5']]:=hsplit_self H5.
-      have[H6'[k6 mrg6']]:=hsplit_self H6.
+      have[H5'[k5 mrg5']]:=split_self H5.
+      have[H6'[k6 mrg6']]:=split_self H6.
       have[_ wr5']:=wr_merge_inv mrg5' wr7.
       have[_ wr6']:=wr_merge_inv mrg6' wr8.
       exists Hx. exists H2. exists n.[m2,m1/]. exists (n'.[n'0,m'0/]).
@@ -489,25 +446,25 @@ Proof with eauto 7 using era_type, resolve, dyn_step, key, merge, hmrg_setmU, hm
         { apply: resolve_subst...
           econstructor...
           econstructor.
-          apply: hmrg_sym mrg5'.
+          apply: merge_sym mrg5'.
           all: eauto.
           constructor... }
         { apply: resolve_subst...
           econstructor...
           econstructor.
-          apply: hmrg_sym mrg5'.
+          apply: merge_sym mrg5'.
           all: eauto.
           constructor... }
         { apply: resolve_subst...
           econstructor...
           econstructor.
-          apply: hmrg_sym mrg5'.
+          apply: merge_sym mrg5'.
           all: eauto.
           constructor... }
         { apply: resolve_subst...
           econstructor...
           econstructor.
-          apply: hmrg_sym mrg5'.
+          apply: merge_sym mrg5'.
           all: eauto.
           constructor... } }
       { apply: star1.
@@ -520,46 +477,37 @@ Proof with eauto 7 using era_type, resolve, dyn_step, key, merge, hmrg_setmU, hm
         constructor... } } }
   { move=>Γ Δ A B m m' n n' t _ erm ihm ern ihn H1 H2 H H' z z' e1 e2 rs wr mrg st; subst.
     inv rs; inv st.
+    have[<-_]:=merge_size mrg.
     have[wr1 wr2]:=wr_merge_inv mrg wr.
     destruct t.
-    { exists (setm H1 l (APair m0 n0 U, U)).
-      exists (setm H2 l (APair m0 n0 U, U)).
+    { exists (APair m0 n0 U :U H1).
+      exists (APair m0 n0 U :U H2).
       exists (APair m n U).
       exists (APair m' n' U).
-      rsplit...
-      { econstructor.
-        rewrite/free setmE eq_refl. rsplit.
-        apply: resolve_wkU.
+      repeat split...
+      { econstructor...
         constructor...
-        by have[]:=hmrg_none mrg H12. }
+        apply: resolve_wkU...
+        apply: resolve_wkU... }
       { have//=nfm':=nf_typing erm.
         have//=nfn':=nf_typing ern.
-        have//nfm0:=resolve_wr_nfi H9 wr1 nfm'.
-        have//nfn0:=resolve_wr_nfi H10 wr1 nfn'.
-        apply: wr_merge.
-        apply: hmrg_setmU...
-        move=>x. have:=wr1 x. rewrite setmE. by case: eqP.
-        move=>x. have:=wr2 x. rewrite setmE. by case: eqP. }
-      { apply: pad_setm.
-        by have[]:=hmrg_none mrg H12. } }
-    { exists (setm H1 l (APair m0 n0 L, L)).
-      exists (H2).
+        constructor...
+        have//:=resolve_wr_nfi H9 wr1 nfm'.
+        have//:=resolve_wr_nfi H10 wr1 nfn'. } }
+    { exists (APair m0 n0 L :L H1).
+      exists (_: H2).
       exists (APair m n L).
       exists (APair m' n' L).
-      rsplit...
-      { econstructor.
-        rewrite/free setmE eq_refl. rsplit.
-        rewrite remm_setm.
+      repeat split...
+      { econstructor...
         constructor...
-        by have[]:=hmrg_none mrg H12. }
+        apply: resolve_wkN...
+        apply: resolve_wkN... }
       { have//=nfm':=nf_typing erm.
         have//=nfn':=nf_typing ern.
-        have//nfm0:=resolve_wr_nfi H9 wr1 nfm'.
-        have//nfn0:=resolve_wr_nfi H10 wr1 nfn'.
-        apply: wr_merge.
-        apply: hmrg_setmL...
-        move=>x. have:=wr1 x. rewrite setmE. by case: eqP.
-        exact: wr2. } } }
+        constructor...
+        have//:=resolve_wr_nfi H9 wr1 nfm'.
+        have//:=resolve_wr_nfi H10 wr1 nfn'. } } }
   { move=>Γ Δ A B m m' t erm ihm H1 H2 H H' z z' e1 e2 rs wr mrg st; subst.
     inv rs; inv st.
     { have[H1'[H2'[x'[y'[wrx[wr'[pd[mrg'[rd1 rd2]]]]]]]]]:=
@@ -641,9 +589,9 @@ Theorem ptr_sr H H' x y z z' A :
   exists x' y', H' ; x' ~ y' ~ z' : A /\ wr_heap H' /\ x ~>>* x' /\ y ~>>* y'.
 Proof with eauto.
   move=>wrx wr st.
-  have[H0[k mrg]]:=hsplit_self H.
+  have[H0[k mrg]]:=split_self H.
   have[H1'[H2'[x'[y'[wrx'[wr'[pd[mrg'[rd1 rd2]]]]]]]]]:=ptr_srX wrx wr mrg st.
   have k':=pad_key pd k.
-  have e:=hmrg_pureR mrg' k'. subst.
+  have e:=merge_pureR mrg' k'. subst.
   exists x'. exists y'...
 Qed.
