coq_bak/sta_valid.v
@@ -1,0 +1,223 @@
+From mathcomp Require Import ssreflect ssrbool eqtype ssrnat seq.
+From Coq Require Import ssrfun Classical Utf8.
+Require Export AutosubstSsr ARS sta_inv.
+
+Set Implicit Arguments.
+Unset Strict Implicit.
+Unset Printing Implicit Defensive.
+
+Theorem sta_valid Γ m A : Γ ⊢ m : A -> exists s l, Γ ⊢ A : Sort s l.
+Proof with eauto using sta_type.
+  move=>ty. elim: ty=>{Γ m A}...
+  { move=>Γ x A wf hs.
+    apply: sta_wf_ok... }
+  { move=>Γ A B m s tym [t[l tyB]].
+    have wf:=sta_type_wf tyB. inv wf.
+    exists s. exists (maxn l0 l)... }
+  { move=>Γ A B m s tym [t[l tyB]].
+    have wf:=sta_type_wf tyB. inv wf.
+    exists s. exists (maxn l0 l)... }
+  { move=>Γ A B m n s tym[s0[l/sta_pi0_inv[t[l1[l2[tyB/sort_inj[e1 e2]]]]]]]tyn _; subst.
+    exists t. exists l1. apply: sta_esubst...
+    by autosubst. }
+  { move=>Γ A B m n s tym[s0[l/sta_pi1_inv[t[l1[l2[tyB/sort_inj[e1 e2]]]]]]]tyn _; subst.
+    exists t. exists l1. apply: sta_esubst...
+    by autosubst. }
+  { move=>Γ A B C m n s t l tyC _ tym _ _ _.
+    have//={}tyC:=sta_subst tyC tym. exists s. exists l... }
+  { move=>Γ A B C m n s t l tyC _ tym _ _ _.
+    have//={}tyC:=sta_subst tyC tym. exists s. exists l... }
+  { move=>Γ A B m n t _[s[lA tyA]]_[r[lB tyB]]. exists t. exists (maxn lA lB)... }
+  { move=>Γ A B m t _ [s[l/sta_with_inv[s0[r[l1[l2[tyA _]]]]]]]. exists s0. exists l1... }
+  { move=>Γ A B m t _ [s[l/sta_with_inv[s0[r[l1[l2[_[tyB _]]]]]]]]. exists r. exists l2... }
+  { move=>Γ A m tym[s[l tyA]]. exists U. exists l... }
+  { move=>Γ A B H P m n s l tyB _ tyH _ tyP[r[l0 tyI]].
+    have[_[tym[tyn _]]]:=sta_id_inv tyI. exists s. exists l.
+    replace (Sort s l) with (Sort s l).[P,n/] by autosubst.
+    apply: sta_substitution...
+    repeat constructor; asimpl... }
+Qed.
+
+Lemma sta_lam0_invX Γ A1 A2 B C m s1 s2 t l :
+  Γ ⊢ Lam0 A1 m s1 : C ->
+  C === Pi0 A2 B s2 ->
+  (A2 :: Γ) ⊢ B : Sort t l ->
+  (A2 :: Γ) ⊢ m : B.
+Proof with eauto.
+  move e:(Lam0 A1 m s1)=>n tyL.
+  elim: tyL A1 A2 B m s1 s2 t l e=>//{Γ C n}.
+  { move=>Γ A B m s tym _ A1 A2 B0 m0
+      s1 s2 t l[e1 e2 e3]/pi0_inj[eq1[eq2 e4]]tyB0; subst.
+    have wf:=sta_type_wf tym. inv wf.
+    have wf:=sta_type_wf tyB0. inv wf.
+    apply: sta_ctx_conv.
+    apply: conv_sym...
+    exact: H4.
+    apply: sta_conv...
+    apply: sta_ctx_conv... }
+  { move=>Γ A B m s l eq1 tym ihm tyB ihB A1 A2 B0 m0
+      s1 s2 t e eq2 tyB0; subst.
+    apply: ihm...
+    apply: conv_trans... }
+Qed.
+
+Lemma sta_lam1_invX Γ A1 A2 B C m s1 s2 t l :
+  Γ ⊢ Lam1 A1 m s1 : C ->
+  C === Pi1 A2 B s2 ->
+  (A2 :: Γ) ⊢ B : Sort t l ->
+  (A2 :: Γ) ⊢ m : B.
+Proof with eauto.
+  move e:(Lam1 A1 m s1)=>n tyL.
+  elim: tyL A1 A2 B m s1 s2 t l e=>//{Γ C n}.
+  { move=>Γ A B m s tym _ A1 A2 B0 m0
+      s1 s2 t l[e1 e2 e3]/pi1_inj[eq1[eq2 e4]]tyB0; subst.
+    have wf:=sta_type_wf tym. inv wf.
+    have wf:=sta_type_wf tyB0. inv wf.
+    apply: sta_ctx_conv.
+    apply: conv_sym...
+    exact: H4.
+    apply: sta_conv...
+    apply: sta_ctx_conv... }
+  { move=>Γ A B m s l eq1 tym ihm tyB ihB A1 A2 B0 m0
+      s1 s2 t e eq2 tyB0; subst.
+    apply: ihm...
+    apply: conv_trans... }
+Qed.
+
+Lemma sta_lam0_inv Γ m A1 A2 B s1 s2 :
+  Γ ⊢ Lam0 A2 m s2 : Pi0 A1 B s1 -> (A1 :: Γ) ⊢ m : B.
+Proof with eauto.
+  move=>ty.
+  have[t[l/sta_pi0_inv[r[l1[l2[tyB _]]]]]]:=sta_valid ty.
+  apply: sta_lam0_invX...
+Qed.
+
+Lemma sta_lam1_inv Γ m A1 A2 B s1 s2 :
+  Γ ⊢ Lam1 A2 m s2 : Pi1 A1 B s1 -> (A1 :: Γ) ⊢ m : B.
+Proof with eauto.
+  move=>ty.
+  have[t[l/sta_pi1_inv[r[l1[l2[tyB _]]]]]]:=sta_valid ty.
+  apply: sta_lam1_invX...
+Qed.
+
+Lemma sta_pair0_invX Γ m n s C :
+  Γ ⊢ Pair0 m n s : C ->
+  forall A B r t l,
+    C === Sig0 A B r ->
+    Γ ⊢ Sig0 A B r : Sort t l ->
+    s = r /\ Γ ⊢ m : A /\ Γ ⊢ n : B.[m/].
+Proof with eauto.
+  move e:(Pair0 m n s)=>x ty.
+  elim: ty m n s e=>//{Γ C x}.
+  { move=>Γ A B m n t l ty1 _ tym _ tyn _ m0 n0 s[e1 e2 e3]A0 B0 r t0 l0
+      /sig0_inj[e4[e5 e6]]ty2; subst.
+    have[s[r0[l1[l2[ord[tyA0[tyB0/sort_inj[e1 e2]]]]]]]]:=sta_sig0_inv ty2; subst.
+    have tym0:Γ ⊢ m : A0 by apply: sta_conv; eauto.
+    repeat split...
+    apply: sta_conv.
+    apply: sta_conv_subst.
+    all: eauto.
+    apply: sta_esubst...
+    by autosubst. }
+  { move=>Γ A B m s l eq tym ihm _ _ m0 n s0 e A0 B0 r t eq' ty.
+    apply: ihm...
+    apply: conv_trans... }
+Qed.
+
+Lemma sta_pair1_invX Γ m n s C :
+  Γ ⊢ Pair1 m n s : C ->
+  forall A B r t l,
+    C === Sig1 A B r ->
+    Γ ⊢ Sig1 A B r : Sort t l ->
+    s = r /\ Γ ⊢ m : A /\ Γ ⊢ n : B.[m/].
+Proof with eauto.
+  move e:(Pair1 m n s)=>x ty.
+  elim: ty m n s e=>//{Γ C x}.
+  { move=>Γ A B m n t l ty1 _ tym _ tyn _ m0 n0 s[e1 e2 e3]A0 B0 r t0 l0
+      /sig1_inj[e4[e5 e6]]ty2; subst.
+    have[s[r0[l1[l2[ord1[ord2[tyA0[tyB0/sort_inj[e1 e2]]]]]]]]]:=sta_sig1_inv ty2; subst.
+    have tym0:Γ ⊢ m : A0 by apply: sta_conv; eauto.
+    repeat split...
+    apply: sta_conv.
+    apply: sta_conv_subst.
+    all: eauto.
+    apply: sta_esubst...
+    by autosubst. }
+  { move=>Γ A B m s l eq tym ihm _ _ m0 n s0 e A0 B0 r t eq' ty.
+    apply: ihm...
+    apply: conv_trans... }
+Qed.
+
+Lemma sta_pair0_inv Γ A B m n s r :
+  Γ ⊢ Pair0 m n s : Sig0 A B r ->
+  s = r /\ Γ ⊢ m : A /\ Γ ⊢ n : B.[m/].
+Proof with eauto.
+  move=>ty.
+  have[t[l tyS]]:=sta_valid ty.
+  apply: sta_pair0_invX...
+Qed.
+
+Lemma sta_pair1_inv Γ A B m n s r :
+  Γ ⊢ Pair1 m n s : Sig1 A B r ->
+  s = r /\ Γ ⊢ m : A /\ Γ ⊢ n : B.[m/].
+Proof with eauto.
+  move=>ty.
+  have[t[l tyS]]:=sta_valid ty.
+  apply: sta_pair1_invX...
+Qed.
+
+Lemma sta_apair_invX Γ m n s C :
+  Γ ⊢ APair m n s : C ->
+  forall A B r t l,
+    C === With A B r ->
+    Γ ⊢ With A B r : Sort t l ->
+    s = r /\ Γ ⊢ m : A /\ Γ ⊢ n : B.
+Proof with eauto.
+  move e:(APair m n s)=>x ty.
+  elim: ty m n s e=>//{Γ C x}.
+  { move=>Γ A B m n t tym ihm tyn ihn m0 n0 s[e1 e2 e3]A0 B0 r t0 l
+      /with_inj[e4[e5 e6]]ty; subst.
+    have[s[r0[l1[l2[tyA0[tyB0 _]]]]]]:=sta_with_inv ty.
+    repeat split...
+    apply: sta_conv...
+    apply: sta_conv... }
+  { move=>Γ A B m s l eq1 tym ihm _ _ m0 n s0 e A0 B0 r t eq' tyw; subst.
+    apply: ihm...
+    apply: conv_trans... }
+Qed.
+
+Lemma sta_apair_inv Γ m n A B s r :
+  Γ ⊢ APair m n s : With A B r ->
+  s = r /\ Γ ⊢ m : A /\ Γ ⊢ n : B.
+Proof with eauto.
+  move=>ty.
+  have[t[l tyW]]:=sta_valid ty.
+  apply: sta_apair_invX...
+Qed.
+
+Lemma sta_refl_invX Γ n C :
+  Γ ⊢ Refl n : C ->
+  forall A m1 m2 s l,
+    C === Id A m1 m2 ->
+    Γ ⊢ Id A m1 m2 : Sort s l ->
+    Γ ⊢ n : A /\ n === m1 /\ n === m2.
+Proof with eauto.
+  move e:(Refl n)=>x ty.
+  elim: ty n e=>//{Γ x C}.
+  { move=>Γ A m tym ihm n[e1]A0 m1 m2 s l/id_inj[e2[e3 e4]]tyI; subst.
+    have[l1[tym1 _]]:=sta_id_inv tyI.
+    have[l2[r tyA0]]:=sta_valid tym1.
+    repeat split...
+    apply: sta_conv... }
+  { move=>Γ A B m s l eqw tym ihm _ _ n e A0 m1 m2 s0 eq' tyI.
+    apply: ihm...
+    apply: conv_trans... }
+Qed.
+
+Lemma sta_refl_inv Γ A m1 m2 n :
+  Γ ⊢ Refl n : Id A m1 m2 -> Γ ⊢ n : A /\ n === m1 /\ n === m2.
+Proof with eauto.
+  move=>ty.
+  have[s[l tyI]]:=sta_valid ty.
+  apply: sta_refl_invX...
+Qed.
